coq/Utils.v
@@ -7,6 +7,12 @@ Import MonadNotation.
 Local Open Scope list_scope.
 Local Open Scope monad_scope.
 
+Definition list_init {A:Type}: nat -> (nat -> A) -> list A.
+Proof. Admitted. (* TODO *)
+
+Definition fold_left2 {A B C:Type} : (A -> B -> C -> A) -> A -> list B -> list C -> A.
+Proof. Admitted. (* TODO *)
+
 Definition mapi {A B: Type} (f: nat -> A -> B) (l:list A) : list B :=
   let fix map_ n (l:list A) :=
     match l with
@@ -31,3 +37,10 @@ Fixpoint monadic_fold_left
          a' <- f a b ;;
          monadic_fold_left f l a'
      end.
+
+Definition monadic_fold_left2
+  {A B C:Type}
+  {m : Type -> Type}
+  {M : Monad m}
+  : (A -> B -> C -> m A) -> A -> list B -> list C -> m A.
+Proof. Admitted. (* TODO *)
